

Week 7 Problem Set

Induction, Recursion, Complexity Analysis

[Show with no answers] [Show with all answers]

1. (Induction proofs)

a. Prove by induction that $1 \cdot 1! + 2 \cdot 2! + \dots + n \cdot n! = (n+1)! - 1$ for all $n \geq 1$ ($n \in \mathbb{N}$).

b. Given the definition,

$$s_1 = 1$$

$$s_{n+1} = \frac{1}{1+s_n} \quad (n > 1)$$

prove by induction that

$$s_n = \frac{\text{FIB}(n)}{\text{FIB}(n+1)}$$

for all $n \geq 1$ ($n \in \mathbb{N}$).

c. Suppose you would like to conclude that $P(n)$ is true for all $n \geq 0$ ($n \in \mathbb{N}$). For each of the following conditions, determine whether the condition is sufficient to prove this.

- i. $P(0)$ and $\forall n \geq 1 (P(n-1) \Rightarrow P(n+1) \wedge P(n+2))$
- ii. $P(1)$ and $\forall n \geq 0 (P(n+1) \Rightarrow P(n) \wedge P(n+2))$
- iii. $P(0)$ and $P(1)$ and $\forall n \geq 1 (P(n) \wedge P(n+1) \Rightarrow P(n+2))$
- iv. $P(0)$ and $P(1)$ and $\forall n \geq 1 (P(n) \Rightarrow P(n+2))$
- v. $P(0)$ and $P(1)$ and $\forall n \geq 1 (P(n) \Rightarrow P(2 \cdot n) \wedge P(2 \cdot n + 1))$
- vi. $P(0)$ and $P(1)$ and $\forall n \geq 1 (P(2 \cdot n) \Rightarrow P(2 \cdot n - 1) \wedge P(2 \cdot n + 1))$

[hide answer]

a. Base case: $1 \cdot 1! = 1 = (1+1!) - 1$

Inductive step:

$$\begin{aligned} 1 \cdot 1! + 2 \cdot 2! + \dots + n \cdot n! + (n+1) \cdot (n+1)! &= (n+1)! - 1 + (n+1) \cdot (n+1)! \quad \text{by induction hypothesis} \\ &= (1 + (n+1)) \cdot (n+1)! - 1 \\ &= (n+2) \cdot (n+1)! - 1 \\ &= (n+2)! - 1 \quad \text{by definition of } (.)! \end{aligned}$$

b. Base case: $s_1 = 1 = \frac{1}{1} = \frac{\text{FIB}(1)}{\text{FIB}(2)}$

Inductive step:

$$s_{n+1} = \frac{1}{1+s_n} = \frac{1}{1+\frac{\text{FIB}(n)}{\text{FIB}(n+1)}} = \frac{1}{\frac{\text{FIB}(n+1)+\text{FIB}(n)}{\text{FIB}(n+1)}} = \frac{1}{\frac{\text{FIB}(n+2)}{\text{FIB}(n+1)}} = \frac{\text{FIB}(n+1)}{\text{FIB}(n+2)}$$

c. Only conditions ii. and v. suffice:

- i. $P(0)$ and $\forall n \geq 1 (P(n-1) \Rightarrow P(n+1) \wedge P(n+2))$ is not sufficient:
From $P(0)$ it follows that $P(2)$ and $P(3)$, but the case $n = 1$ is not covered.
- ii. $P(1)$ and $\forall n \geq 0 (P(n+1) \Rightarrow P(n) \wedge P(n+2))$ proves $P(n)$ for all $n \geq 0$:
 $P(1)$ implies $P(0)$ and $P(2)$, then $P(2)$ implies $P(3)$, and so on.
- iii. $P(0)$ and $P(1)$ and $\forall n \geq 1 (P(n) \wedge P(n+1) \Rightarrow P(n+2))$ is not sufficient:
The "first" instance of the implication is $P(1) \wedge P(2) \Rightarrow P(3)$, but $P(2)$ is not given.
- iv. $P(0)$ and $P(1)$ and $\forall n \geq 1 (P(n) \Rightarrow P(n+2))$ is not sufficient:
The "first" instance of the implication is $P(1) \Rightarrow P(3)$, hence the case $P(2)$ cannot be derived.
- v. $P(0)$ and $P(1)$ and $\forall n \geq 1 (P(n) \Rightarrow P(2 \cdot n) \wedge P(2 \cdot n + 1))$ proves $P(n)$ for all $n \geq 0$:
 $P(1)$ implies $P(2)$ and $P(3)$, $P(2)$ implies $P(4)$ and $P(5)$, and so on.

- vi. $P(0)$ and $P(1)$ and $\forall n \geq 1 (P(2 \cdot n) \Rightarrow P(2 \cdot n - 1) \wedge P(2 \cdot n + 1))$ is not sufficient:
The "first" instance of the implication is $P(2) \Rightarrow P(1) \wedge P(3)$, but $P(2)$ is not given.

2. (Recursive definitions)

Recall the recursive definition of a rooted tree:

$\langle v; \rangle$ is a tree consisting only of a root node
 $\langle r; T_1, T_2, \dots, T_k \rangle$ is a tree with root r and subtrees T_1, T_2, \dots, T_k at the root ($k \geq 1$)

Prove that in any rooted tree, the number of leaves is one more than the number of nodes with a right sibling.

Hint: This assumes a given order among the children of every node from left to right; see slide 22 (week 7) for an instance of this theorem.

[hide answer]

For a tree T , let $\ell(T)$ and $r(T)$ denote, respectively, the number of leaves and the number of vertices with a right sibling.

Base case:

A tree consisting of just a root has 1 leaf and no vertex with a right sibling:

$$T = \langle v; \rangle \Rightarrow \ell(T) = 1 = 0 + 1 = r(T) + 1$$

Inductive step:

Consider the tree $T = \langle r; T_1, T_2, \dots, T_{k-1}, T_k \rangle$.

- The leaves in T are all the leaves of all the subtrees T_i . Hence, $\ell(T) = \sum_{i=1}^k \ell(T_i)$.
 - The vertices in T with a right sibling are
 - all the vertices with a right sibling in all of the subtrees T_i
 - and the roots of all the subtrees T_1, \dots, T_{k-1} (but not T_k because it is the last child of the root r in tree T).
- Hence, $r(T) = (k - 1) + \sum_{i=1}^k r(T_i)$.

From the induction hypothesis, $\ell(T_i) = r(T_i) + 1$ for all $1 \leq i \leq k$, it follows that

$$\begin{aligned} \ell(T) &= \sum_{i=1}^k \ell(T_i) \\ &= \sum_{i=1}^k (r(T_i) + 1) \quad \text{by induction hypothesis} \\ &= k + \sum_{i=1}^k r(T_i) \\ &= r(T) + 1 \end{aligned}$$

3. (Recurrences)

Recall the recurrence for Mergesort:

- $T(1) = 0$
- $T(n) = 2T(\frac{n}{2}) + (n - 1)$

Prove that $n \cdot (\log_2 n - 1) + 1$ is a valid formula for $T(n)$ for all $n = 2^k$ (with $k \geq 1$).

[hide answer]

Base case: $T(2^1) = 2 \cdot 0 + (2^1 - 1) = 1$; this is the same as $2^1 \cdot (\log_2 2^1 - 1) + 1 = 2 \cdot 0 + 1 = 1$

Inductive step:

$$\begin{aligned} T(2^{k+1}) &= 2 \cdot T(\frac{2^{k+1}}{2}) + (2^{k+1} - 1) && \text{by the recurrence} \\ &= 2 \cdot T(2^k) + (2^{k+1} - 1) \\ &= 2 \cdot (2^k \cdot (\log_2 2^k - 1) + 1) + (2^{k+1} - 1) && \text{by induction hypothesis} \\ &= 2^{k+1} \cdot (\log_2 2^k - 1) + 2 + 2^{k+1} - 1 \\ &= 2^{k+1} \cdot ((\log_2 2^k - 1) + 1) + 1 \\ &= 2^{k+1} \cdot k + 1 \\ &= 2^{k+1} \cdot (\log_2 2^{k+1} - 1) + 1 \end{aligned}$$

4. (Asymptotic running times)

a. Suppose you have the choice between three algorithms:

- i. Algorithm A solves your problem by dividing it into five subproblems of half the size, recursively solving each subproblem, and then combining the solutions in linear time.

- ii. Algorithm B solves problems of size n by recursively solving two subproblems of size $n - 1$ and then combining the solutions in constant time.
- iii. Algorithm C solves problems of size n by dividing them into nine subproblems of size $\frac{n}{3}$, recursively solving each subproblem, and then combining the solutions in $\mathcal{O}(n^2)$ time.

Estimate the running times of each of these algorithms. Which one would you choose?

b. Order the following functions in increasing asymptotic complexity:

- i. $(n - 1) \cdot (n - 2) \cdot \sqrt{n}$
- ii. $\frac{3n}{\sqrt{n+1}}$
- iii. $\sqrt{7n^3 + 3n + 1}$
- iv. $5n^{\log(\log(n))}$
- v. $3n \log(n) + 2n^2$
- vi. $8 + \log(n) \cdot (n - 1)$

[hide answer]

a. C has the best asymptotic running time:

- i. $T(n) = 5 \cdot T(\frac{n}{2}) + \mathcal{O}(n)$. The Master Theorem with $d = 2$, $\alpha = \log_2 5$, $\beta = 1$ implies, since $\alpha > \beta$, that $T(n) = \mathcal{O}(n^{\log_2 5}) = \mathcal{O}(n^{2.322})$.
- ii. $T(n) = 2 \cdot T(n - 1) + \mathcal{O}(1)$. The theorem on linear reductions with $c = 2$, $k = 0$ implies, since $c > 1$, that $T(n) = \mathcal{O}(2^n)$.
- iii. $T(n) = 9 \cdot T(\frac{n}{3}) + \mathcal{O}(n^2)$. The Master Theorem with $d = 3$, $\alpha = 2$, $\beta = 2$ implies, since $\alpha = \beta$, that $T(n) = \mathcal{O}(n^2 \log n)$.

b. The correct ordering is (ii) < (vi) < (iii) < (v) < (i) < (iv), with (ii) having the best and (iv) the worst asymptotic complexity:

- i. $(n - 1) \cdot (n - 2) \cdot \sqrt{n} \in \Theta(n^2 \cdot n^{0.5}) = \Theta(n^{2.5})$
- ii. $\frac{3n}{\sqrt{n+1}} \in \Theta(n \cdot n^{-0.5}) = \Theta(n^{0.5})$
- iii. $\sqrt{7n^3 + 3n + 1} = (7n^3 + 3n + 1)^{0.5} \in \Theta(n^{1.5})$
- iv. $5n^{\log(\log(n))} \in \Theta(n^{\log(\log(n))})$. For sufficiently large n , $\log(\log(n)) > k$ for any given $k \in \mathbb{R}^+$
- v. $3n \log n + 2n^2 \in \Theta(n^2)$
- vi. $(8 + \log(n)) \cdot (n - 1) = 8n + n \log(n) - \log(n) - 8 \in \Theta(n \cdot \log(n))$

5. (Big-Oh)

a. Without using the Master Theorem, give tight big-Oh upper bounds for the divide-and-conquer recurrence $T(1) = 1$; $T(n) = T(\frac{n}{2}) + g(n)$, for $n > 1$, where

- i. $g(n) = 1$
- ii. $g(n) = 2n$
- iii. $g(n) = n^2$

b. For each of the following functions, use the Master Theorem to determine the best upper bound complexity of $T(n)$.

- i. $T(n) = 9 \cdot T(\frac{n}{3}) + 3n(n + 1)$
- ii. $T(n) = 8 \cdot T(\frac{n}{2}) + 8n(n + 1)$
- iii. $T(n) = 8 \cdot T(\frac{n}{2}) + 2n^2(n + 1)$
- iv. $T(n) = 6 \cdot T(\frac{n}{2}) + n^3$
- v. $T(n) = 6 \cdot T(\frac{n}{3}) + n^2$

c. Analyse the complexity of the following recursive algorithm to test whether a number x occurs in an *unordered* list $L = [x_1, x_2, \dots, x_n]$ of size n . Take the cost to be the number of list element comparison operations.

```

Search( $x, L = [x_1, x_2, \dots, x_n]$ ):
  if  $x_1 = x$  then return yes
  else if  $n > 1$  then return Search( $x, [x_2, \dots, x_n]$ )
  else return no

```

- d. Analyse the complexity of the following recursive algorithm to test whether a number x occurs in an *ordered* list $L = [x_1, x_2, \dots, x_n]$ of size n . Take the cost to be the number of list element comparison operations.

```

BinarySearch( $x, L = [x_1, x_2, \dots, x_n]$ ):
  if  $n = 0$  then return no
  else if  $x_{\lceil \frac{n}{2} \rceil} > x$  then return BinarySearch( $x, [x_1, \dots, x_{\lceil \frac{n}{2} \rceil - 1}]$ )
  else if  $x_{\lceil \frac{n}{2} \rceil} < x$  then return BinarySearch( $x, [x_{\lceil \frac{n}{2} \rceil + 1}, \dots, x_n]$ )
  else return yes

```

[hide answer]

- a. Unrolling the recursive definitions:

$$\begin{aligned}
 \text{i. } T(n) &= T\left(\frac{n}{2}\right) + 1 = T\left(\frac{n}{4}\right) + 2 = T\left(\frac{n}{8}\right) + 3 = \dots = T\left(\frac{n}{n}\right) + \log_2 n = \mathcal{O}(\log n) \\
 \text{ii. } T(n) &= 2n + \frac{2n}{2} + \frac{2n}{4} + \frac{2n}{8} + \dots = 2n \cdot \left(1 + \frac{1}{2} + \frac{1}{4} + \frac{1}{8} + \dots\right) = \mathcal{O}(4n) = \mathcal{O}(n) \\
 \text{iii. } T(n) &= n^2 + \left(\frac{n}{2}\right)^2 + \left(\frac{n}{4}\right)^2 + \left(\frac{n}{8}\right)^2 + \dots = n^2 \cdot \left(1 + \frac{1}{4} + \frac{1}{16} + \frac{1}{64} + \dots\right) = \mathcal{O}\left(\frac{4}{3}n^2\right) = \mathcal{O}(n^2)
 \end{aligned}$$

- b. The Master Theorem requires to determine the parameters d , α and β and compare α and β :

- $d = 3$, $\alpha = 2$ and $\beta = 2$. From $\alpha = \beta$ it follows that the solution is $\mathcal{O}(n^2 \cdot \log(n))$.
- $d = 2$, $\alpha = 3$ and $\beta = 2$. From $\alpha > \beta$ it follows that the solution is $\mathcal{O}(n^3)$.
- $d = 2$, $\alpha = 3$ and $\beta = 3$. From $\alpha = \beta$ it follows that the solution is $\mathcal{O}(n^3 \cdot \log(n))$.
- $d = 2$, $\alpha = 2.585$ and $\beta = 3$. From $\alpha < \beta$ it follows that the solution is $\mathcal{O}(n^3)$.
- $d = 3$, $\alpha = 1.631$ and $\beta = 2$. From $\alpha < \beta$ it follows that the solution is $\mathcal{O}(n^2)$.

- c. The worst case is when the element occurs last in the list (or not at all). Let $T(n)$ be the total cost of running *Search* ($x, [x_1, \dots, x_n]$) in this case.

- if $x_1 = x$ then return yes **cost = 1** (one list element comparison)
- else if $n > 1$ then return *Search*($x, [x_2, \dots, x_n]$) **cost = $T(n - 1)$** (recursive call with list size $n - 1$)
- else return no **cost = 0**

This can be described by the recurrence $T(1) = 1$; $T(n) = 1 + T(n - 1)$ with the solution $T(n) = \mathcal{O}(n)$.

- d. Again, the worst case is when the element occurs last in the list (or is larger than the last element). Let $T(n)$ be the total cost of running *BinarySearch*($x, [x_1, \dots, x_n]$) in this case.

- if $n = 0$ then return no **cost = 0**
- else if $x_{\lceil \frac{n}{2} \rceil} > x$ then return *BinarySearch*($x, [x_1, \dots, x_{\lceil \frac{n}{2} \rceil - 1}]$) **cost = 1** (one list element comparison; this condition is never satisfied in the assumed worst case that x is the largest element in the list)
- else if $x_{\lceil \frac{n}{2} \rceil} < x$ then return *BinarySearch*($x, [x_{\lceil \frac{n}{2} \rceil + 1}, \dots, x_n]$) **cost = $1 + T(\lfloor \frac{n}{2} \rfloor)$** (one comparison plus cost of recursive call with the second half of the list)
- else return yes **cost = 0**

This can be described by the recurrence $T(0) = 0$; $T(n) = 2 + T\left(\frac{n}{2}\right)$ with the solution $T(n) = \mathcal{O}(\log n)$.

6. Challenge Exercise

Prove by induction that every connected graph $G = (V, E)$ must satisfy $e(G) \geq v(G) - 1$.

Hint: You can use the fact from a previous lecture that $\sum_{v \in V} \deg(v) = 2 \cdot e(G)$.

[hide answer]

Base case: A graph with $v(G) = 1$ node is connected, has $e(G) = 0$ edges and hence satisfies $e(G) \geq v(G) - 1$.

Inductive step (proof by contradiction):

Consider graph G with $v(G) \geq 2$ nodes such that $e(G) < v(G) - 1$. We will show that G is not connected. From the lecture we know that $\sum_{v \in V} \deg(v) = 2e(G) < 2v(G) - 2$ (according to the assumption). It follows that there is at least one vertex $v_0 \in V$ with $\deg(v_0) \leq 1$, since otherwise $\sum_{v \in V} \deg(v) \geq 2v(G)$.

- If $\deg(v_0) = 0$ then G is not connected and we are done.
- If $\deg(v_0) = 1$, consider the graph G' obtained by removing v_0 and its only connecting edge from G . It follows that $e(G') < v(G') - 1$ since $e(G') = e(G) - 1$, $v(G') = v(G) - 1$ and $e(G) < v(G) - 1$. By the induction hypothesis, G' cannot be connected, since $e(G') \not\geq v(G') - 1$. But then neither can be G : if v and w are vertices with no path between them in G' then adding v_0 doesn't help.

Assessment

After you have solved the exercises, go to [COMP9020 20T1 Quiz Week 7](#) to answer 5 quiz questions on this week's problem set (Exercises 1-5 only) and lecture.

The quiz is worth 2.5 marks.

There is no time limit on the quiz once you have started it, but the deadline for submitting your quiz answers is **Thursday, 9 April 10:00:00am**.

Please continue to respect the **quiz rules**:

Do ...

- use your own best judgement to understand & solve a question
- discuss quizzes on the forum only **after** the deadline on Thursday

Do not ...

- post specific questions about the quiz **before** the Thursday deadline
- agonise too much about a question that you find too difficult